##### Exercise 3.3.1
Let $f:X\to Y$, $g:X\to Y$, $h: X \to Y$, $j : Y \to Z$ be functions.
- Reflexive
We know that for all $x \in X$ $f(x) = f(x)$ thus $f = f$.
- Symmetry
If $f = g$ then we know that for all $x \in X$ $f(x) = g(x)$ thus $g(x) = f(x)$, and by definition 3.3.7 $g= f$.
- Transitive
We need to show that if $f = g$ and $g = h$ then $f = h$. We know that for all $x \in X$ $f(x) = g(x)$ and $g(x) = h(x)$, thus $f(x) = h(x)$ showing that $f = h$.
- Substitution
Let $\tilde{f} = f$ and $\tilde{j} = j$ be functions. We need to prove that $j\circ f = \tilde{j}\circ \tilde{f}$. By definition 3.3.10 it will suffice to show that for all $x\in X$ $j(f(x)) = \tilde{j}(\tilde{f}(x))$. We already know that for all $x \in X$ $f(x) = \tilde{f}(x)$ thus we can say that $\tilde{j}(\tilde{f}(x)) = \tilde{j}(f(x))$ and since we know that for all $y \in Y$ $j(y) = \tilde{j}(y)$, thus $\tilde{j}(f(x)) = j(f(x))$ completing the proof.
##### Exercise 3.3.2
- If $f : X\to Y$ and $g : Y\to Z$ are injective prove that $g\circ f$ is also injective.
Since we know that $f$ and $g$ are injective, by definition 3.1.14 we know that for all $x,x' \in X, x\neq x' \iff f(x) \neq f(x')$ and we know that for all $y,y' \in Y, y \neq y' \iff g(y) \neq g(y')$, thus for all $f(x),f(x') \in Y, f(x) \neq f(x') \iff g(f(x)) \neq g(f(x'))$. Combining these two statements we can see that for all $x,x' \in X, x\neq x' \iff g(f(x)) \neq g(f(x'))$ proving that $g\circ f$ is injective.
- If $f : X\to Y$ and $g : Y\to Z$ are surjective prove that $g\circ f$ is also surjective.
We already know that for all $y \in Y$, there exists $x\in X$ such that $f(x) = y$. And we know that for all $z\in Z$, there exists $y \in Y$ such that $g(y) = z$, and because we know that every $y \in Y$ can be written as $f(x)$ where $x \in X$, we can say for all $z\in Z$, there exists $f(x) \in Y, x \in X$ such that $g(f(x)) = z$, thus completing the proof.  
##### Exercise 3.3.3
Let $f : \emptyset \to A$ be an empty function
- We know that function $f$ is always injective as the statement "for all $x,x' \in \emptyset, x \neq x' \implies f(x) \neq f(x')$" is vacuously true because by axiom 3.2 no object is an element of the empty set.
- For function $f$ to be surjective, for every $y \in A$, there exists $x\in \emptyset$ such that $f(x) = y$. But since we know from axiom 3.2 that no object is an element of the empty set, the only way for that statement to be true is $A = \emptyset$ because if that was the case the statement would be vacuously true.
- We have shown that $f$ is always injective and $f$ is injective iff $A = \emptyset$, thus $f$ is bijective iff $A = \emptyset$.
##### Exercise 3.3.4
Let $f : X\to Y, \tilde{f} : X\to Y, g : Y \to Z, \tilde{g} : Y \to Z$ be functions.
- If $g\circ f = g\circ \tilde{f}$ and $g$ is injective, then $f = \tilde{f}$
We know that since $g$ is injective so by definition 3.3.14 for every $y,y' \in Y$ $y \neq y' \implies g(y) \neq g(y')$, or we can say that $g(y) = g(y') \implies y = y'$. We know that $g \circ f = g\circ \tilde{f}$, thus from definition 3.3.10 and definition 3.3.14 for every $f(x),\tilde{f}(x) \in Y, g(f(x)) = g(\tilde{f}(x)) \implies f(x) = \tilde{f}(x)$ and using definition 3.3.7 we can show that $f = \tilde{f}$.
If $g$ was not injective we could have a case like this:
Suppose that $X = \{1,2\}$, $Y = \{1,2\}$, $Z = \{1\}$ and that $f(x) := x,\tilde{f}(1) := 2, \tilde{f}(2) := 1,g(x) := 1$. We know that $g\circ f(1) = 1, g\circ f(2) = 1$ and $g\circ \tilde{f}(1) = 1, g\circ \tilde{f}(2) = 1$, thus $g\circ f = g\circ \tilde{f}$ by definition 3.3.7, but we know from definition 3.3.7 that $f \neq \tilde{f}$ as $f(1) = 1$ and $\tilde{f}(1) = 2$, and with this we have shown that the statement would not be true if $g$ wasn't injective.
- If $g\circ f = \tilde{g} \circ f$ and f is surjective, then $g = \tilde{g}$
We know that $g \circ f = \tilde{g} \circ f$, implies that for every $f(x) \in Y$, $g(f(x)) = \tilde{g}(f(x))$, and we know that f is surjective so by definition 3.3.17 for every $y \in Y$, there exists $x\in X$ such that $f(x) = y$, thus for every $y \in Y$, $g(y) = \tilde{g}(y)$. By definition 3.3.7 $g = \tilde{g}$.
If $f$ was not surjective we could have a case like this:
Suppose that $X = \{1\}, Y = \{1,2\}, Z =\{1,2,3\}$, and that $f(1) := 1, g(x) := x, \tilde{g}(1) := 1, \tilde{g}(2) := 3$. We know that $g \circ f(1) = 1$ and $\tilde{g} \circ f(1) = 1$, thus $g\circ f = \tilde{g} \circ f$ by definition 3.3.7, but we also know from definition 3.3.7 that $g \neq \tilde{g}$ as $g(2) = 2$ and $\tilde{g}(2) = 3$, and with this we have shown that the statement would not be true if $f$ wasn't surjective. 
##### Exercise 3.3.5
Let $f : X \to Y$ and $g : Y \to Z$ be functions
- If $g\circ f$ is injective then $f$ is injective
We know that $g\circ f$ is injective, then by definition 3.3.14 and definition 3.3.10 for every $x,x' \in X$, $x \neq x' \implies g(f(x)) \neq g(f(x'))$. From definition 3.3.7 we know that for all $x \in X$, $x = x' \implies g(x) = g(x')$, thus if we assume that there exists $x,x' \in X$ such that  $x \neq x'$ and $f(x) = f(x')$ for the sake of contradiction, then $g(f(x)) = g(f(x'))$, but this would contradict the fact that $g\circ f$ is injective. Now that we know for all $x,x' \in X$, $x \neq x'\implies f(x) \neq f(x')$ by definition 3.3.14 $f$ is injective.
Let's say that $X = \{1\}, Y = \{1,2\}, Z = \{1\}$, and $f(1) := 1, g(x) = 1$. We know that by definition 3.3.14  $g \circ f$ is injective because $g\circ f(1) = 1$ and there are no other elements in the domain. But as we can see $g(0) = g(1) = 1$, thus by definition 3.1.14 $g$ is not injective, and we have shown that $g \circ f$ being injective does not imply $g$ is also injective.
- If $g\circ f$ is surjective then $g$ is surjective
We know that if $g \circ f$ is surjective, then by definition 3.3.17 for every $z \in Z$, there exists $x \in X$ such that $g(f(x)) = z$, and using definition 3.3.12 we can say that for every $z \in Z$, there exists $f(x) \in Y$ such that $g(f(x)) = z$, thus by definition 3.3.17 $g$ is surjective.  
Let's say that $X = \{1\}, Y = \{1,2\}, Z = \{1\}$, and $f(1) := 1, g(x) = 1$. We know that by definition 3.3.17 $g \circ f$ is surjective because $g \circ f(1) = 1$ which covers all of the elements of $Z$, but we also know that $f$ is not surjective because there is no $x \in X$ such that $f(x) = 2$, thus by definition 3.3.17 $f$ is not surjective, and we have shown that $g \circ f$ being surjective does not imply that $f$ is also surjective.
##### Exercise 3.3.6
Let $f:X\to Y$ be a bijective function and $f^{-1} : Y \to X$ be it's inverse function. From remark 3.3.24 we know that for every $y \in Y$, there is exactly one $x$ such that $f(x) = y$ and we know that the value of $x$ is denoted as $f^{-1}(y)$. Thus using the definition of inverse function we know that $f(f^{-1}(y)) = y$, and since $f(x) = y$ and $f^{-1}(y) = x$ we know that $f^{-1}(f(x)) = x$. If we look at the definition of inverse function once again we can see that the inverse of the function $f^{-1}(y) = x$ is the function $(f^{-1})^{-1}(x) = y$ which is the same function as $f$. 
##### Exercise 3.3.7
We know that $f$ maps every $x\in X$ to a different $y\in Y$ and since $g$ maps every different $y\in Y$ to a different $z\in Z$, the function $g\circ f$ maps every $x\in X$ to a different $z\in Z$ thus it is a bijective function.
Let's say we have sets $X$, $Y$ and $Z$ and we have functions $f: X\to Y$, $g: Y\to Z$ such that $f(x) = y$, $g(y) = z$ and $g(f(x)) = z$. Let $x\in X$, $y\in Y$ and $z\in Z$ be any object such that $f(x) = y$ and $g(y) = z$. We know that $g\circ f(x) = z$, $(g\circ f)^{-1}(z) = x$, $f^{-1}(y) = x$ and $g^{-1}(z) = y$. We can see that $f^{-1}\circ g^{-1}(z) = x$ thus $(g\circ f)^{-1} = f^{-1}\circ g^{-1}$. 
##### Exercise 3.3.8
- From the definition of function composition we know that $\iota_{Y\to Z}\circ\iota_{X\to Y}$ is a function that is defined from the domain $X$ to the range $Z$. We also know that $\iota_{X\to Y}(x) = x$ and $\iota_{Y\to Z}(x) = x$ thus the composite function $\iota_{Y\to Z}\circ\iota_{X\to Y}(x) = x$ which shows that it is the identity function $\iota_{X\to Z}$.
- We know that $\iota_{A\to A}(a) = a$ where $a\in A$ thus by the axiom of replacement $f(\iota_{A\to A}(a)) = f(a)$. Using a similar logic we can also show that $f(a) = \iota_{B\to B}(f(a))$.
- Let $a$ and $b$ be objects such that $a\in A$,$b\in B$ and $f(a) = b$. We can also see that $a = f^{-1}(b)$. By the axiom of replacement we can say that $f(a) = b\iff f(f^{-1}(b)) = b$, thus $f\circ f^{-1}$ is the identity function $\iota_{B\to B}$. Using a similar argument we can show that $f^{-1}\circ f=\iota_{A\to A}$.
- Let's say that $h:X\cup Y\to Z$ is a function such that for all $x$ where $x\in X$ and $x\in X\cup Y$, $h(x) = f(x)$ and for all $y$ where $y\in Y$ and $y\in X\cup Y$, $h(y) = g(y)$. Since we know that all elements in $X\cup Y$ is either an element of $X$ or an element of $Y$ from the axiom of pairwise union and since the two sets are disjoint we can safely say that we have sufficiently declared a function $h$, and since we have defined $h$ to be equal to the function $f$ when the input is an element of $X$ and vice versa we can safely say that $h\circ\iota_{X\to X\cup Y} = f$ and $h\circ\iota_{Y\to X\cup Y} = g$. 
  Now we need to show that the function $h$ is unique for functions $f$ and $g$. Let's say that $\tilde{h}:X\cup Y\to Z$ be another function such that $\tilde{h}\circ\iota_{X\to X\cup Y} = f$ and $\tilde{h}\circ\iota_{Y\to X\cup Y} = g$ , we need to show that $h = \tilde{h}$ and for that we need to show $h(a) = \tilde{h}(a), \forall a \in X\cup Y$. We can inspect this in two cases. Either $a \in X$ or $a\in Y$. When $a\in X$ we know that $h(x) = f(x) = \tilde{h}(x)$ and when $a\in Y$ we know that $h(a)=g(a)=\tilde{h}(a)$ thus $h=\tilde{h}$ completing the proof.