##### Exercise 3.5.1
$\newcommand{\and}{\text{ and }}\newcommand{\or}{\text{ or }}\newcommand{\N}{\mathbb{N}}\newcommand{\pp}{\verb!++!}$Let $(x, y)$ be an ordered pair and we'll assume the definition of ordered pair to be $(x,y) := \{\{x\},\{x,y\}\}$. We need to prove that $(x,y)=(x',y')\iff(x=x'\text{ and }y=y')$. By our definition $(x,y)=(x',y') \iff \{\{x\},\{x,y\}\}=\{\{x'\},\{x',y'\}\}$. Since both sets have two elements there are two ways of them being equal. Either $\{x\} = \{x',y'\} \text{ and }\{x,y\}=\{x'\}$ or $\{x\} = \{x'\}\text{ and }\{x,y\}=\{x',y'\}$. In the first case we can see that the sets $\{x\}$ and $\{x',y'\}$ are equal iff $x = x' = y'$ and the sets $\{x,y\}$ and $\{x'\}$ are equal iff $x=y=x'$ thus we can see that for the first case the ordered pairs are equal iff $x=y=x'=y'$. In the second case the sets $\{x\}$ and $\{x'\}$ are equal iff $x=x'$ and for the other sets we can assume that $x=x'$ since otherwise it won't matter if they are equal or not. The sets $\{x,y\}$ and $\{x',y'\}$ are equal iff $y=y'\text{ or }(x=y' \text{ and } x'=y)$ but since $x=x'$ the second statement implies the first one and we can omit it. Thus $(x,y) = (x',y')\iff(x=x'=y=y'\text{ or }(x=x'\text{ and }y=y'))$ but since the first case is a more special version of the second case we can omit it and we arrive at $(x,y)=(x',y')\iff x=x'\text{ and }y=y'$ completing the proof.
Let $(x,y)$ be an ordered pair and we'll assume the definition of ordered pair to be $(x,y) := \{x,\{x,y\}\}$. We need to prove that $(x,y)=(x',y')\iff(x=x'\text{ and }y=y')$. Using a similar argument we can see that the second case does not change. However we need to look at the first case again. Let's assume that $x=\{x',y'\}\text{ and }x'=\{x,y\}$, but since we proved that two sets $A$ and $B$ cannot contain each other in [[Chapter 3.2#Exercise 3.2.2]] we know that if $x'\in x$ then $x$ must not be an element of $x'$ thus a contradiction. This doesn't change the outcome but we know that the first case is a contradiction.
##### Exercise 3.5.2
The exercise has merely stated the definition of function equality thus it is indeed correct. If we write them in more conventional function notation it is easier to see this fact:
Let $A = \{i\in \mathbb{N}:1\le i\le n\}$ and $B$ be sets and let $x:A\to B$ and $y: A\to B$ be functions. By the definition of function equality $x=y\iff x(i)=y(i)\text{ for all }i\in A$. Since we know all the elements in the set $A$ we can write this as $x=y\iff x(i)=y(i)\text{ for all }1 \le i\le n$ and using the alternative syntax for these functions it becomes the statement in the exercise $(x_i)_{1\le i\le n}=(y_i)_{1\le i\le n} \iff x_i = y_i \text{ for all }1\le i\le n$.

Let $(X_i)_{1\le i\le n}$ be an ordered n-tuple of sets. From the axiom of union we know that the set of all elements of all the sets in the n-tuple $(X_i)_{1\le i\le n}$ is a set and we'll call it $A$. Let $B$ be the set of all partial functions from  $\{i\in \mathbb{N}\:1\le i\le n\}\to A'$ where $A'$ is any subset of the set $A$. We can show that this set exists using a similar argument to the [[Chapter 3.4#Exercise 3.4.7]]. Let $P(f)$ be a property pertaining to the function $f$. $P(f)$ is true iff $f$ is surjective and if $f(x)\in X_i$ then $x' \neq x \iff f(x')\notin X_i$. Using the axiom of specification we can say that the set $\{f\in B: P(f) \text{ is true }\}$ exists and is the same set as $\Pi_{1\le i\le n}X_i$.
##### Exercise 3.5.3
- $(x,y) = (x,y)\iff(x=x\and y=y)$
- $(x,y) = (x',y')\iff(x=x'\and y=y')\iff(x'=x\and y'=y)\iff(x',y')=(x,y)$
- $(x,y) = (x',y')\iff(x=x'\and y=y')$
  $(x',y')=(x'',y'')\iff (x'=x''\and y'=y'')$
  thus $(x=x''\and y=y'')\iff(x,y)=(x'',y'')$
- $(x_i)_{1\le i\le n} = (x_i)_{1\le i\le n}\iff(x_i=x_i\text{ for all }1\le i\le n)$
- $(x_i)_{1\le i\le n} = (x'_i)_{1\le i\le n}\iff(x_i=x'_i\text{ for all }1\le i\le n)\iff(x'_i=x_i\text{ for all }1\le i\le n)\iff(x'_i)_{1\le i\le n}=(x_i)_{1\le i\le n}$
- $(x_i)_{1\le i\le n} = (x'_i)_{1\le i\le n}\iff(x_i=x'_i\text{ for all }1\le i\le n)$ and 
  $(x'_i)_{1\le i\le n}=(x''_i)_{1\le i\le n}\iff(x'_i=x''_i\text{ for all }1\le i\le n)$
  thus $(x_i=x''_i\text{ for all }1\le i\le n)\iff(x_i)_{1\le i\le n}=(x''_i)_{1\le i\le n}$
##### Exercise 3.5.4
By the definition of Cartesian product and the axiom pairwise union we can say that $(x,y)\in A\times(B\cup C)\iff (x\in A \text{ and } (y\in B \text{ or }y\in C)$ and the statement on the right is equivalent to $((x\in A \text{ and }y\in B)\text{ or }(x\in A \text{ and }y\in C))$.
Similarly we can say that $(x,y)\in(A\times B)\cup(A\times C)\iff ((x\in A \text{ and }y\in B)\text{ or }(x\in A \text{ and }y\in C))$ thus from the definition of set equality we have shown that $A\times(B\cup C) = (A\times B)\cup(A\times C)$.

By the definition of Cartesian product and the definition of pairwise intersection we can say that $(x,y)\in A\times(B\cap C)\iff (x\in A \text{ and } y\in B \text{ and }y\in C)$.
Similarly we can say that $(x,y)\in(A\times B)\cap(A\times C)\iff ((x\in A \text{ and }y\in B)\text{ and }(x\in A \text{ and }y\in C))$ and if we remove the repetition and the unnecessary parenthesis we get $(x\in A\text{ and }y\in B\text{ and }y\in C)$ thus from the definition of set equality we have shown that $A\times(B\cap C) = (A\times B)\cap(A\times C)$.

By the definition of Cartesian product and the definition of set difference we can say that $(x,y)\in A\times(B\setminus C)\iff (x\in A \text{ and } y\in B \text{ and }y\notin C)$.
Similarly we can say that $(x,y)\in(A\times B)\setminus(A\times C)\iff ((x\in A \text{ and }y\in B)\text{ and }(x\notin A \text{ or }y\notin C))$ and since we know that $(x\in A\text{ and }x\notin A)$ is always false we can remove it thus leaving us with $(x\in A\text{ and }y\in B\text{ and }y\notin C)$. From the definition of set equality we have shown that $A\times(B\setminus C) = (A\times B)\setminus(A\times C)$.
##### Exercise 3.5.5
By the definition of Cartesian product and the definition of pairwise intersection we can see that $(x,y)\in (A\times B)\cap(C\times D)\iff (x\in A\and y\in B)\and(x\in C\and y\in D)$. Using a similar logic we can say that $(x,y)\in(A\cap C)\times(B\cap D)\iff (x\in A \and x\in C)\and(y\in B\and y\in D)$ and it is trivial to see that these two statements are equivalent thus by the definition of set equality $(A\times B)\cap(C\times D)=(A\cap C)\times(B\cap D)$.

Using a similar logic and the axiom of pairwise union we can see that $(x,y)\in(A\times B)\cup(C\times D)\iff((x\in A\and y\in B)\or(x\in C\and y\in D))$, and $(x,y)\in(A\cup C)\times(B\cup D)\iff ((x\in A\or x\in C)\and (y\in B\or y\in D))$.  These two are clearly not equal and we can show it by providing an ordered pair like this: $(x,y)$ where $(x\in A\and x\notin C\and y \notin B\and y\in D)$. We know that $(x,y) \in (A\cup C)\times(B\cup D)$ but $(x,y)\notin(A\times B)\cup(C\times D)$ thus they are not equal.

Using a similar logic and the definition of set difference we can see that $(x,y)\in(A\times B)\setminus(C\times D)\iff((x\in A\and y\in B)\and(x\notin C\or y\notin D))$, and $(x,y)\in(A\setminus C)\times(B\setminus D)\iff ((x\in A\and x\notin C)\and (y\in B\and y\notin D))$. These two are clearly not equal and we can show it by giving an ordered pair like this: $(x,y)$ where $(x\in A\and x\notin C\and y\in B \and y\in D)$. We know that $(x,y)\in(A\times B)\setminus(C\times D)$ but $(x,y)\notin(A\setminus C)\times(B\setminus D)$.
##### Exercise 3.5.6
From the definition of subset we can see that $A\times B\subseteq C\times D\iff((x,y)\in A\times B\implies (x,y)\in C\times D)$. Using the definition of Cartesian product we can see that $A\times B \subseteq C\times D\iff (x\in A\and y\in B\implies x\in C\and y\in D)$. Since we know that all of the sets are non-empty this statement cannot be vacuously true thus $A\times B\subseteq C\times D$ iff every element of $A$ is also be an element $C$ and every element of $B$ is also an element of $D$ or in other words $A\times B\subseteq C\times D\iff(A\subseteq C\and B\subseteq D)$ thus completing the proof. 
If either $A$ or $B$ was an empty set the statement $(x\in A\and y\in B\implies x\in C\and y\in D)$ would be vacuously true thus what the other set is irrelevant. Because of this if $A=\emptyset$ then it doesn't matter what $B$ is since $A \times B = \emptyset$ and vice versa, thus if the sets can be the empty set it is not necessarily true that $(A\subseteq C\and B\subseteq D)$.
##### Exercise 3.5.7
We can construct the function $h:Z\to X\times Y$ to be $h(z) = (f(z),g(z))$ where $z\in Z$ and since we know that $f:Z\to X$ and $g:Z\to Y$ are functions then the function $h$ exists.
Now we need to make sure the function $h$ is unique for functions $f$ and $g$. Let's say that $\tilde{h}:Z\to X\times Y$ is a function such that $\pi_{X\times Y\ to X}\circ\tilde{h} = f$ and $\pi_{X\times Y\to Y}\circ\tilde{h} = g$. We can see that $\pi_{X\times Y\to X}\circ h = f = \pi_{X\times Y\to X}\circ\tilde{h}$ and  $\pi_{X\times Y\to Y}\circ h = g = \pi_{X\times Y\to Y}\circ\tilde{h}$ thus the function $h$ is unique.
##### Exercise 3.5.8
By the definition of n-fold Cartesian product we know that the i'th element in every product must be an element from $X_i$ but since $X_i$ is empty no tuple can satisfy the condition thus $\Pi^n_{i=1}X_i \text{ is empty}$.
##### Exercise 3.5.9
From the axiom of union and the definition of intersection we know that $y\in (\bigcup_{\alpha\in I}A_\alpha)\cap(\bigcup_{\beta\in J}B_\beta)\iff((y\in A_\alpha\text{ for some }\alpha\in I)\and (y\in B_\beta\text{ for some }\beta\in J))$. Following a similar logic we can also see that $y\in \bigcup_{(\alpha,\beta)\in I\times J}(A_\alpha\cap B_\beta)\iff(y\in A_\alpha\and y\in B_\beta \text{ for some }(\alpha,\beta)\in I\times J)$, and using the definition of Cartesian product we can see that $(y\in A_\alpha\and y\in B_\beta \text{ for some }(\alpha,\beta)\in I\times J)\iff((y\in A_\alpha\text{ for some }\alpha\in I)\and (y\in B_\beta\text{ for some }\beta\in J))$ thus completing the proof.
##### Exercise 3.5.10
From the definition of function equality $f=\tilde{f}\iff f(x)=\tilde{f}(x)\text{ for all }x\in X$, thus by the definition of ordered pair equality we can see that $f=\tilde{f}\iff(x,f(x))=(x,\tilde{f}(x))\text{ for all }x\in X$ and using the definition of set equality we can say that $f=\tilde{f}\iff\{(x,f(x)):x\in X\}=\{(x,\tilde{f}(x)):x\in X\}$.

We know that for each $x\in X$ there exists exactly one element in $\{y\in Y:(x,y)\in G\}$ thus for every element $x\in X$. Let $f:X\to Y$ be a function such that for every $x\in X$, $(x, f(x))\in G$. We know this function exists because of the way the set $G$ was constructed and from the definition we defined for the graph of a function we can see that $G$ is the graph of $f$.
##### Exercise 3.5.11
From definition of Cartesian product and lemma 3.4.9 we know the set $\{Z: Z\subseteq (X\times Y)\}$. By the axiom of specification we also know that the set $A = \{G\in Z:\forall x\in X\text{ the set }\{y\in Y:(x,y)\in G\}\text{ has exactly one element}\}$ exists and using a similar logic to [[#Exercise 3.5.10]] we can see that all of the sets in the set $A$ is the graph of a unique function thus by the replacement axiom we can replace the graphs with their functions. This set would be equivalent to the power set $Y^X$ completing the proof.
##### Exercise 3.5.12
Let $c$ be a natural number and $f:\N\times \N\to \N$. Let $a_0:\{0\}\to \N$ be the function that $a_0(0) = c$. It is trivial to see that this function exists and is unique to the natural number $c$. Let's assume inductively that the function $a_N:\{n\in\N:n\le N\}\to\N$ exists and we need to show that the function $a_{N\pp}:\{n\in\N:n\le N\pp\}\to\N$ exists such that for all $n\in\{n\in\N:n\le N\}, a_{N\pp}(n)=a_N(n)$ and $a_{N\pp}(N\pp)=f(N,a_{N}(N))$. We can see that for all values of $n\le N$ the function $a_{N\pp}$ is uniquely defined by our inductive hypothesis and we also know that the function $f$ every input in $\N\times \N$ to a unique output in $\N$ we can see that the function $a_{N\pp}$ not only exists but is unique for function $f$ and natural number $c$ thus closing the induction.
TODO!!
##### Exercise 3.5.13
TODO!!